finished Encrypt-then-mac example, crypto code review needed

examples/crypto/EtM.AE.fst
@@ -12,14 +12,13 @@ open CoreCrypto
 
 module CPA = EtM.CPA
 module MAC = EtM.MAC
+module P   = EtM.Plain
 
 type log_t (r:rid) = Monotonic.Seq.log_t r (CPA.msg * CPA.cipher * MAC.tag)
 
-//val mac_log: r:rid -> log_t r -> MAC.log_t r
 
 noeq type key = 
   | Key:  #region:rid -> ke:CPA.key { extends (CPA.Key.region ke) region  } -> km:MAC.key { extends (MAC.Key.region km) region /\  (disjoint( CPA.Key.region ke) (MAC.Key.region km)) } -> log:log_t region -> key 
-  (* currently needs flag --__temp_no_proj EtM.AE *)
 
 
 let invariant (h:t) (k:key) = 
@@ -74,80 +73,67 @@ let keygen parent =
   let log = alloc_mref_seq region createEmpty in
   Key #region ke ka log
 
-let invariant2 (h:t) (k:key) = 
-  let log = m_sel h k.log in
-  let mac_log = m_sel h (MAC.Key.log k.km) in
-  let cpa_log = m_sel h (CPA.Key.log k.ke) in
-  Map.contains h k.region /\
-  Map.contains h (MAC.Key.region k.km) /\
-  Map.contains h (CPA.Key.region k.ke) /\
-  Seq.length log = Seq.length mac_log /\
-  Seq.length mac_log = Seq.length cpa_log /\ 
-  (* (forall (i:int). indexable log i ==> *)
-  (*   (let m1,t = Seq.index mac_log i in *)
-  (*   let m2,c = Seq.index cpa_log i in *)
-  (*   m1 = c /\ *)
-  (*   Seq.index log i = (m2,c,t) /\ *)
-  (*   True *)
-  (*   ) ) /\ *)
-  True
-
 
 val encrypt: k:key -> m:EtM.Plain.plain -> ST cipher
   (requires (fun h0 -> invariant h0 k))
   (ensures  (fun h0 c h1 ->
-    (let ilog = m_sel h0 k.log in
-     let n = Seq.length ilog in
+    (let log0 = get_log h0 k in
+     let log1 = get_log h1 k in
+     let n = Seq.length log0 in
        modifies (Set.singleton k.region)  h0 h1
-     /\ m_contains k.log h1
-     /\ m_sel h1 k.log == snoc ilog (m, fst c, snd c)
+     /\ log1 == snoc log0 (m, fst c, snd c)
      /\ witnessed (at_least n (m, fst c, snd c) k.log)
-     /\ (invariant h0 k ==> invariant2 h1 k)))) //invariant h1 k
+     /\ (invariant h0 k ==> invariant h1 k))))
 
-
+#set-options "--initial_fuel 0 --max_fuel 0 --initial_ifuel 1 --max_ifuel 1 --z3timeout 100"
 let encrypt k plain =
-  m_recall k.log;
   let h0 = ST.get () in
-  cut (Seq.length (get_mac_log h0 k) = Seq.length (get_cpa_log h0 k));
-  assert (disjoint (MAC.Key.region k.km) (CPA.Key.region k.ke));
-  assert (Map.contains h0 (MAC.Key.region k.km));
   let c = CPA.encrypt k.ke plain in
-//  let c = createBytes 1 0z in //with this instead of encrypt the length checks work
-//  assert (disjoint (MAC.Key.region k.km) (CPA.Key.region k.ke));
-  m_recall (MAC.Key.log k.km);
-  m_recall (CPA.Key.log k.ke);
-  let h1 = ST.get () in
-  (* assert (Map.contains h0 (MAC.Key.region k.km)); *)
-  (* assert (Map.contains h0 (CPA.Key.region k.ke)); *)
-  (* assert (Seq.length (get_mac_log h1 k) = Seq.length (get_mac_log h0 k)); *)
   let t = MAC.mac k.km c in
-  let h2 = ST.get () in
-  assert (disjoint (MAC.Key.region k.km) (CPA.Key.region k.ke));
-  assert (Seq.length (get_mac_log h2 k) = Seq.length (get_mac_log h1 k)+1);
-  assert (Seq.length (get_mac_log h2 k) = Seq.length (get_mac_log h0 k)+1);
-  m_recall (MAC.Key.log k.km);
-  m_recall (CPA.Key.log k.ke);
-  cut (Seq.index (get_mac_log h2 k) (Seq.length (get_mac_log h2 k)-1) = (c,t));
-  cut (Seq.index (get_cpa_log h2 k) (Seq.length (get_cpa_log h2 k)-1) = (plain,c));
-  (* cut (Seq.length (get_cpa_log h2 k) = Seq.length (get_cpa_log h0 k)+1); *)
-  (* cut (Seq.length (get_mac_log h2 k) = Seq.length (get_mac_log h0 k)+1); *)
-  cut (Seq.length (get_mac_log h2 k) = Seq.length (get_cpa_log h2 k));
   write_at_end k.log (plain,c,t);
-  (* lemma_slice_snoc (get_log h k) 0 (Seq.length (get_log h k));  *)
-  (* lemma_slice_snoc (get_mac_log h k) 0 (Seq.length (get_mac_log h k)); *)
-  (* lemma_slice_snoc (get_cpa_log h k) 0 (Seq.length (get_cpa_log h k)); *)
-  let h = ST.get () in
-  (* cut (Seq.index (get_mac_log h k) (Seq.length (get_mac_log h k)-1) = (c,t)); *)
-  (* cut (Seq.index (get_cpa_log h k) (Seq.length (get_cpa_log h k)-1) = (plain,c)); *)
-  cut (Seq.index (get_log h k) (Seq.length (get_log h k)-1) = (plain,c,t)); 
+  let h1 = ST.get () in
+  //following assertions seem no longer needed
+  (* cut (Seq.length (get_log h1 k) = (Seq.length (get_log h0 k)) + 1);   *)
+  (* cut (Seq.length (get_mac_log h1 k) = Seq.length (get_cpa_log h1 k)); *)
+  (* cut (Seq.length (get_mac_log h1 k) = Seq.length (get_log h1 k));   *)
+  (* cut (Seq.index (get_mac_log h1 k) (Seq.length (get_mac_log h1 k)-1) = (c,t)); *)
+  (* cut (Seq.index (get_cpa_log h1 k) (Seq.length (get_cpa_log h1 k)-1) = (plain,c)); *)
+  (* cut (Seq.index (get_log h1 k) (Seq.length (get_log h1 k)-1) = (plain,c,t));  *)
+  assert
+  ( let log  = get_log h1 k in
+    let mac_log = get_mac_log h1 k in
+    let cpa_log = get_cpa_log h1 k in
+    (forall (i:int). indexable log i ==>
+      (let m1,t = Seq.index mac_log i in
+      let m2,c = Seq.index cpa_log i in
+      m1 = c /\
+      Seq.index log i = (m2,c,t) /\
+      True)
+    )
+    );
   (c, t)
-   
   
-val decrypt: k:key -> c:cipher -> option EtM.Plain.plain
+
+assume AE_needs_CMA: (MAC.uf_cma <==> P.ind_cpa)
+
+val decrypt: k:key -> c:cipher -> ST (option EtM.Plain.plain)
+  (requires (fun h0 -> invariant h0 k))
+  (ensures (fun h0 p h1 -> 
+    modifies_none h0 h1 /\ 
+    (invariant h0 k ==> invariant h1 k)
+  ))
 let decrypt k (c,tag) =
   if MAC.verify k.km c tag
   then (
-  admit();
-  Some(CPA.decrypt k.ke c) 
+    if (MAC.uf_cma) then 
+      (
+      (* let h = ST.get () in *)
+      (* assert ( is_Some (seq_find (fun mt -> mt = (c,tag)) (get_mac_log h k) ) ); *)
+      Some(CPA.decrypt k.ke c)
+      )
+    else 
+      (
+      Some(CPA.decrypt k.ke c) 
+      )
   )
-  else None
+  else ( None )
